Complete soundness proof with new instructions

Hoare/HoareTripleForBasicBlocks.thy
@@ -400,8 +400,8 @@ inductive triple_inst_storage :: "network \<Rightarrow> pred \<Rightarrow> pos_i
        \<and>* program_counter k \<and>* storage idx w \<and>* gas_pred g \<and>*  account_existence c existence
        \<and>* continuing \<and>* rest)
       (k, Storage SLOAD)
-      (block_number_pred bn \<and>* stack_height (h + 1) \<and>* stack h w
-       \<and>* program_counter (k + 1) \<and>* storage idx w \<and>* gas_pred (g - Gsload net)
+      (program_counter (k + 1) \<and>* block_number_pred bn \<and>* stack_height (h + 1) \<and>* stack h w
+       \<and>* storage idx w \<and>* gas_pred (g - Gsload net)
        \<and>*  account_existence c existence \<and>* continuing \<and>* rest)"
 
 inductive triple_inst_info :: "pred \<Rightarrow> pos_inst \<Rightarrow> pred \<Rightarrow> bool" where
